verif/btrees_sep.v
@@ -268,6 +268,13 @@ Fixpoint partial_cursor_correct {X:Type} (c:cursor X) (n:node X) (root:node X): 
   | (n',i)::c' => (partial_cursor_correct c' n' root) /\ (nth_node i n' = Some n)
   end.
 
+Lemma partial_correct_index : forall (X:Type) (c:cursor X) n i n' root,
+    partial_cursor_correct ((n,i)::c) n' root -> idx_to_Z i < Z.of_nat (numKeys n).
+Proof.
+  intros. unfold partial_cursor_correct in H. destruct H.
+  apply nth_node_some in H0. auto.
+Qed.
+
 (* Complete cursor is correct and points to (keyval k v x) *)
 Definition complete_cursor_correct {X:Type} (c:cursor X) k v x (root:node X): Prop :=
   match c with
@@ -277,6 +284,13 @@ Definition complete_cursor_correct {X:Type} (c:cursor X) k v x (root:node X): Pr
                  | ip ii => partial_cursor_correct c' n root /\ nth_entry ii n = Some (keyval X k v x)
                  end
   end.
+
+Lemma complete_correct_index : forall {X:Type} (c:cursor X) n i k v x root,
+    complete_cursor_correct ((n,i)::c) k v x root -> idx_to_Z i < Z.of_nat (numKeys n).
+Proof.
+  intros. unfold complete_cursor_correct in H. destruct i.
+  omega. destruct H. apply nth_entry_some in H0. simpl. omega.
+Qed.
 
 (* Cursor is complete and correct for relation *)
 Definition complete_cursor_correct_rel {X:Type} (c:cursor X) (rel:relation X): Prop :=
