verif/verif_currnode.v
@@ -22,8 +22,7 @@ Proof.
   destruct r as [root prel].
   pose (r:=(root,prel)).
   destruct c as [|[n i] c'].
-  { destruct H; inv H; inv H1. inv H. } (* cursor can't be empty *)
-
+  { destruct H; inv H; inv H2. inv H. } (* cursor can't be empty *)
   unfold cursor_rep. Intros anc_end. Intros idx_end.
   assert_PROP( is_pointer_or_null (getval n)).
   { assert(subnode (currNode ((n,i)::c') r) (get_root r)).
@@ -34,11 +33,11 @@ Proof.
       unfold relation_rep. rewrite subnode_rep with (n:=n) by auto. entailer!. }
   forward.                      (* t'1=cursor->level *)
   forward.                      (* t'2=cursor->ancestors[t'1] *)
-  { entailer!. apply partial_complete_length with (r:=r). auto. }
+  { entailer!. apply partial_complete_length with (r:=r). unfold r. auto. auto. }
   { entailer!. 
     rewrite app_Znth1. rewrite app_Znth2.
     rewrite Zlength_cons. rewrite Zsuccminusone. rewrite Zlength_rev. rewrite Zlength_map.
-    rewrite Zlength_map. assert(Zlength c'-Zlength c' = 0) by omega. rewrite H8.
+    rewrite Zlength_map. assert(Zlength c'-Zlength c' = 0) by omega. rewrite H9.
     rewrite Znth_0_cons. auto.
     rewrite Zlength_cons. rewrite Zsuccminusone. rewrite Zlength_rev. rewrite Zlength_map.
     rewrite Zlength_map. omega.
@@ -48,7 +47,7 @@ Proof.
   + rewrite app_Znth1.
     rewrite Zlength_cons. rewrite app_Znth2.
     rewrite Zlength_rev. rewrite Zlength_map. rewrite Zlength_map.
-    assert((Z.succ (Zlength c') - 1 - Zlength c') = 0) by omega. rewrite H9.
+    assert((Z.succ (Zlength c') - 1 - Zlength c') = 0) by omega. rewrite H10.
     rewrite Znth_0_cons. auto.
     rewrite Zlength_rev. rewrite Zlength_map. rewrite Zlength_map. omega.
     rewrite Zlength_app. rewrite Zlength_rev. rewrite Zlength_map. rewrite Zlength_map.
