verif/verif_findindex.v
@@ -16,6 +16,36 @@ Require Import btrees_sep.
 Require Import btrees_spec.
 Require Import index.
 
+Lemma FCI_increase: forall X (le:listentry X) key i,
+    idx_to_Z i <= idx_to_Z (findChildIndex' le key i).
+Proof.
+  intros. generalize dependent i.
+  induction le; intros.
+  - simpl. omega.
+  - destruct e; simpl.
+    * destruct (key.(k_) <? k.(k_)). omega.
+      eapply Z.le_trans with (m:=idx_to_Z (next_index i)). rewrite next_idx_to_Z. omega.
+      apply IHle.
+    * destruct (key.(k_) <? k.(k_)). omega.
+      eapply Z.le_trans with (m:=idx_to_Z (next_index i)). rewrite next_idx_to_Z. omega.
+      apply IHle.
+Qed.
+
+Lemma FRI_increase: forall X (le:listentry X) key i,
+    idx_to_Z i <= idx_to_Z (findRecordIndex' le key i).
+Proof.
+  intros. generalize dependent i.
+  induction le; intros.
+  - simpl. omega.
+  - destruct e; simpl.
+    * destruct (key.(k_) <=? k.(k_)). omega.
+      eapply Z.le_trans with (m:=idx_to_Z (next_index i)). rewrite next_idx_to_Z. omega.
+      apply IHle.
+    * destruct (key.(k_) <=? k.(k_)). omega.
+      eapply Z.le_trans with (m:=idx_to_Z (next_index i)). rewrite next_idx_to_Z. omega.
+      apply IHle.
+Qed.
+
 Lemma body_findChildIndex: semax_body Vprog Gprog f_findChildIndex findChildIndex_spec.
 Proof.
   start_function.
@@ -55,29 +85,47 @@ Proof.
       forward.                  (* i=0 *)
       gather_SEP 0 1 2 3 4 5. replace_SEP 0 (btnode_rep n). { entailer!. Exists ent_end0. entailer!. } deadvars!.
       
-{ forward_loop (EX i:Z, PROP(i<=idx_to_Z (findChildIndex n key)) LOCAL(temp _i (Vint(Int.repr i)); temp _node pn; temp _key (key_repr key)) SEP(btnode_rep n))
-                   break:(EX i:Z, PROP(i=idx_to_Z (findChildIndex n key)) LOCAL(temp _i (Vint(Int.repr i)); temp _node pn; temp _key (key_repr key)) SEP(btnode_rep n)).
+{ forward_loop (EX i:Z, PROP(i<=Z.of_nat(numKeys n) -1) LOCAL(temp _i (Vint(Int.repr i)); temp _node pn; temp _key (key_repr key)) SEP(btnode_rep n))
+                   break:(EX i:Z, PROP(i=Z.of_nat(numKeys n) -1) LOCAL(temp _i (Vint(Int.repr i)); temp _node pn; temp _key (key_repr key)) SEP(btnode_rep n)).
 
   - Exists 0. entailer!.
-    rewrite key_unsigned_repr in H. rewrite key_unsigned_repr in H.
-    assert (key.(k_) <? k.(k_) = false). admit.   (* true from H *)
-    rewrite H2.
-    admit.                      (* OK because fCI' is called with ip 0 *)
+    destruct (Pos.of_succ_nat (numKeys_le le')).
+    apply Pos2Z.is_nonneg. apply Pos2Z.is_nonneg. omega.
+    
+    (* rewrite key_unsigned_repr in H. rewrite key_unsigned_repr in H. *)
+    (* apply Z.ge_le in H. *)
+    (* apply Fcore_Zaux.Zlt_bool_false in H. rewrite H. *)
+    (* replace 0 with (idx_to_Z (ip O)). *)
+    (* apply FCI_increase. auto. *)
   - Intros i.
     rewrite unfold_btnode_rep. unfold n. Intros ent_end1.
     forward.                    (* t'5=node->numKeys *)
     gather_SEP 0 1 2 3 4 5 6. replace_SEP 0 (btnode_rep n). { entailer!. Exists ent_end1. entailer!. } 
-    assert((numKeys (btnode val ptr0 (cons val (keychild val k n0) le') false First Last pn)) = S (numKeys_le le')). simpl. auto.
+    assert((numKeys (btnode val ptr0 (cons val (keychild val k n0) le') false First Last pn)) = S (numKeys_le le')). { simpl. auto. }
     rewrite H3.
     forward_if.
-    + entailer!. admit.         (* le not to large *)
-    + forward.                  (* skip *)
+    + entailer!.
+      clear -H1. unfold node_wf in H1. simpl in H1.
+      rewrite Zpos_P_of_succ_nat.
+      rewrite Int.signed_repr.      
+      rewrite Int.signed_repr by rep_omega. rep_omega.
+      rep_omega.
+    + forward.                  (* rest of the loop *)
       admit.                    (* TODO *)
     + forward.                  (* break *)
-      Exists (idx_to_Z (findChildIndex n key)). entailer!.
+      Exists (Z.of_nat (numKeys n) -1). entailer!.      
       admit.                    (* TODO *)
-  - Intros i.
-    admit. }                    (* TODO *)
+  - Intros i.                   (* after the loop *)
+    rewrite unfold_btnode_rep. unfold n. Intros ent_end1.
+    forward.                    (* t'2=node->numKeys *)
+    forward.                    (* return *)
+    + entailer!. rewrite Zpos_P_of_succ_nat. unfold node_wf in H1. simpl in H1. clear -H1.
+      rewrite Int.signed_repr. rewrite Int.signed_repr.
+      rewrite Zsuccminusone. rep_omega. rep_omega. rep_omega.
+    + Exists ent_end1.
+      entailer!.
+      (* prove that numKeys-1 is FCI *)
+      admit. }
 Admitted.
 
 
@@ -87,49 +135,5 @@ Proof.
   forward.                      (* i=0 *)
   destruct n as [ptr0 le isLeaf First Last pn].
   pose (n:= btnode val ptr0 le isLeaf First Last pn). fold n.
-  forward_if (PROP ( ) LOCAL (temp _i (Vint (Int.repr 0)); temp _node pn; temp _key (Vint (Int.repr key))) SEP (btnode_rep n)).
-  - apply denote_tc_test_eq_split.
-    admit.                      (* valid pointer *)
-    entailer!.
-  - forward.                    (* skip *)
-    entailer!.
-  - assert_PROP(False). unfold btnode_rep. entailer!.
-    admit.                      (* offset_val 20 p = nullval should be a contradiction? *)
-    contradiction.
-  - rewrite unfold_btnode_rep. unfold n. Intros.
-    forward.                    (* t'5=node->numKeys *)
-    gather_SEP 0 1 2 3. replace_SEP 0 (btnode_rep n). { entailer!. }
-    { forward_if(PROP ( ) LOCAL (temp _t'5 (Vint (Int.repr (Z.of_nat (numKeys (btnode val ptr0 le isLeaf First Last pn))))); temp _i (Vint (Int.repr 0)); temp _node pn; temp _key (Vint (Int.repr key))) SEP (btnode_rep n)).
-      - forward.                (* skip *)
-        entailer!.
-      - admit.
-        (* contradiction in H1 *)
-      - rewrite unfold_btnode_rep. unfold n. Intros.
-        forward.                (* t'4=node->numKeys *)
-        forward_if.
-        + forward.              (* return *)
-          entailer!.
-          assert(le= nil val). admit. (* true from H1 *)
-          rewrite H5. simpl. auto.
-        + forward.              (* skip *)
-          forward.              (* i=0 *)
-          gather_SEP 0 1 2 3. replace_SEP 0 (btnode_rep n). { entailer!. } deadvars!.
-{ forward_loop (EX i:Z, (PROP (i<= Z.of_nat (numKeys_le le))
-     LOCAL (temp _i (Vint (Int.repr i)); temp _node pn; temp _key (Vint (Int.repr key)))
-     SEP (btnode_rep n)))
-               break:(EX i:Z, (PROP (i= Z.of_nat(numKeys_le le))
-     LOCAL (temp _i (Vint (Int.repr i)); temp _node pn; temp _key (Vint (Int.repr key)))
-     SEP (btnode_rep n))).
-  - Exists 0. entailer!.
-  - Intros i. rewrite unfold_btnode_rep. unfold n. Intros.
-    forward.                    (* t'3=node->numKeys *)
-    forward_if.
-    + entailer!. admit.
-    + forward. admit.
-    + forward. admit.
-  - Intros i. rewrite unfold_btnode_rep. unfold n. Intros.
-    forward.                    (* t'1=node->numKeys *)
-    forward.                    (* return *)
-    entailer!.
-    admit.                      (* loop invariant isn't strong enough *) } }
+  forward_if (PROP ( ) LOCAL (temp _i (Vint (Int.repr 0)); temp _node pn; temp _key (key_repr key)) SEP (btnode_rep n)).
 Admitted.
