verif/verif_isvalid.v
@@ -22,7 +22,6 @@ Lemma body_isValid: semax_body Vprog Gprog f_isValid isValid_spec.
 Proof.
   start_function.
   forward_call(r,c,pc).      (* t'1=entryIndex(cursor) *)
-  admit.
   forward_call(r,c,pc).      (* t'2=currNode *)
   assert (COMPLETE: complete_cursor c r) by auto.
   unfold complete_cursor in H. destruct H.
@@ -34,15 +33,16 @@ Proof.
   assert (n = currNode c r). simpl. auto.
   simpl in H0. destruct i as [|ii]. contradiction.
   apply complete_cursor_subnode in H. unfold get_root in H. simpl in H.
+  assert (SUBNODE: subnode n root) by auto.
   unfold relation_rep. unfold r.
-  rewrite subnode_rep with (n:=currNode c (root,numRec,depth,prel)) by auto. Intros.
+  rewrite subnode_rep with (n:=currNode c (root,prel)) by auto. Intros.
   rewrite unfold_btnode_rep at 1.
-  assert(currNode c r = currNode c (root,numRec,depth,prel)). auto.
-  destruct (currNode c (root,numRec,depth,prel)) as [ptr0 le b First Last pn]. Intros.
-  pose (currnode:= btnode val ptr0 le b First Last pn).
+  assert(currNode c r = currNode c (root,prel)). auto.
+  destruct (currNode c (root,prel)) as [ptr0 le b First Last pn]. Intros.
+  pose (currnode:= btnode val ptr0 le b First Last pn). Intros ent_end.
   forward.                      (* t'5=t'2->numKeys *)
   gather_SEP 2 3 4 5. replace_SEP 0 (btnode_rep (currNode c r)).
-  { rewrite unfold_btnode_rep. rewrite H2. entailer!. }
+  { rewrite unfold_btnode_rep. rewrite H4. entailer!. Exists ent_end. entailer!. }
   
   forward_if  (PROP ( )
      LOCAL (temp _t'5 (Vint (Int.repr (Z.of_nat (numKeys (btnode val ptr0 le b First Last pn)))));
@@ -50,51 +50,59 @@ Proof.
      temp _cursor pc; temp _t'3 (Val.of_bool (negb (isValid c r))) (* new local *))
      SEP (btnode_rep (currNode c r); malloc_token Tsh trelation prel;
      data_at Tsh trelation
-       (getval root, (Vint (Int.repr (Z.of_nat numRec)), Vint (Int.repr (Z.of_nat depth)))) prel;
+       (getval root, (Vint (Int.repr (Z.of_nat (get_numrec (root,prel)))), Vint (Int.repr (Z.of_nat (get_depth (root,prel)))))) prel;
      btnode_rep (btnode val ptr0 le b First Last pn) -* btnode_rep root;
-     cursor_rep c (root, numRec, depth, prel) pc)).
+     cursor_rep c (root, prel) pc)).
 
   - forward_call(r,c,pc).
     + unfold r. cancel. unfold relation_rep.
       cancel.
       change_compspecs btrees.CompSpecs.
-      cancel. eapply derives_trans. fold r. rewrite H2. apply wand_frame_elim. cancel.
+      cancel. eapply derives_trans. fold r. rewrite H4. apply wand_frame_elim. cancel.
     + unfold relation_rep. unfold r. Intros.
       rewrite subnode_rep with (n:=currNode c r) by auto.
-      rewrite H2. fold r.
+      rewrite H4. fold r.
       rewrite unfold_btnode_rep at 1.
-      Intros. rewrite H2.
+      Intros. rewrite H4. Intros ent_end0.
       forward.                  (* t'6=t'4->LastLeaf *)
-      * autorewrite with norm. entailer!. destruct Last; simpl; auto.
+      * entailer!. destruct Last; simpl; auto.
       * forward.                (* t'3=(tbool) (t'6==1) *)
         entailer!.
-        { unfold isValid.
-          rewrite H2. destruct Last; simpl; auto.
-          admit.                (* true from H3 *)
-        }
-        assert(n = currNode c r). simpl. auto. rewrite H13.
-        rewrite unfold_btnode_rep. rewrite H2.
-        entailer!. fold r. apply derives_refl.
+        { unfold isValid. rewrite H4. destruct Last; simpl; auto.
+          assert(0 <= Z.of_nat (numKeys_le le) <= Int.max_unsigned).
+          { unfold root_wf in H1. unfold get_root in H1. simpl in H1.
+          apply H1 in SUBNODE. unfold node_wf in SUBNODE. unfold numKeys in SUBNODE.
+          rewrite H3 in SUBNODE. rewrite H4 in SUBNODE. rep_omega. }
+          apply repr_inj_unsigned in H5. apply Nat2Z.inj in H5.
+          rewrite H5. rewrite Nat.eqb_refl. simpl. auto.
+          unfold complete_cursor in COMPLETE. destruct COMPLETE.
+          unfold complete_cursor_correct_rel in H16.
+          destruct (getCEntry ((n,ip ii)::c')); try inv H16.
+          destruct e; try inv H16.
+          apply complete_correct_index in H16. rewrite H3, H4 in H16. simpl in H16.
+          rep_omega. auto. }
+        assert(n = currNode c r). simpl. auto. rewrite H15.
+        rewrite unfold_btnode_rep. rewrite H4.
+        entailer!. Exists ent_end0. entailer!. fold r. apply derives_refl.
   - forward.                    (* t'3=0 *)
     entailer!.
-    unfold isValid. rewrite H2.
+    unfold isValid. rewrite H4.
     destruct Last; auto.
     assert(index.index_eqb (entryIndex c) (index.ip (numKeys_le le)) = false).
-    { unfold index.index_eqb.
-      unfold entryIndex. unfold c.
-      admit.                    (* true from H3 *)
-    }
-    rewrite H9. auto.
+    { unfold c. simpl.
+      destruct (ii =? numKeys_le le)%nat eqn:HEQ; auto.
+      apply beq_nat_true in HEQ. subst ii. contradiction. }      
+    rewrite H11. auto.
     apply derives_refl.
   - gather_SEP 0 3. replace_SEP 0 (btnode_rep root).
     { entailer!. rewrite unfold_btnode_rep at 1. assert(n = currNode c r) by (simpl; auto).
-      rewrite H6. rewrite H2. apply wand_frame_elim. }
+      rewrite H8. rewrite H4. apply wand_frame_elim. }
     gather_SEP 0 1 2. replace_SEP 0 (relation_rep r).
     { entailer!. apply derives_refl. }
     forward_if.
-    + forward. fold c. entailer!. fold r. rewrite H3. auto.
-    + forward. fold c. entailer!. fold r. rewrite H3. auto.
-Admitted.
+    + forward. fold c. entailer!. fold r. rewrite H5. auto.
+    + forward. fold c. entailer!. fold r. rewrite H5. auto.
+Qed.
   
 Lemma body_RL_CursorIsValid: semax_body Vprog Gprog f_RL_CursorIsValid RL_CursorIsValid_spec.
 Proof.
